Refinery/Term/Extrinsic/Minimal.lean
@@ -76,6 +76,19 @@ theorem SDeriv.wt {Γ : Ctx? α} {A : Ty α} {a : Term φ (Ty α)} (D : Γ ⊢�
 def SDeriv.bv_at {Γ : Ctx? α} {A : Ty α} {n : ℕ} (D : Γ ⊢ₛ (.bv (φ := φ) n) : A)
   : Γ.SAt ⟨A, 1⟩ n := match D with | .bv hv => hv
 
+-- theorem SDeriv.ueq {Γ Γ' : Ctx? α} {A A' : Ty α} {a : Term φ (Ty α)}
+--   (D : Γ ⊢ₛ a : A) (D' : Γ' ⊢ₛ a : A') (hΓ : Γ.TyEq Γ')
+--   : Γ.UEq Γ' := by induction D generalizing Γ' A' with
+--   | bv hv => cases D' with | bv hv' =>
+--     apply hv.ueq_of_ty_eq; assumption; cases hv.ty_eq_out hΓ hv'; assumption; simp
+--   | let₁ => sorry
+--   | unit => sorry
+--   | pair => sorry
+--   | let₂ => sorry
+--   | case => sorry
+--   | iter => sorry
+--   | _ => cases D'; apply_assumption <;> assumption
+
 end Term
 
 end Refinery
